BSWLean/Conversion.lean
@@ -10,30 +10,22 @@ This file provides all necessary definitions to make this conversion.
 
 /-- Takes assignment `ρ`, variable `v` and produce a literal contradicting `ρ`, if `v` happens
 to be in the preimage of `ρ`. -/
+@[simp]
 def Assignment.negVariable {vars} (ρ : Assignment vars) (v : Variable) : Option (Literal vars) :=
   if h_v_mem_vars : v ∈ vars then
-    if ρ v h_v_mem_vars then
-      some (Variable.toNegLiteral v h_v_mem_vars)
-    else
-      some (Variable.toLiteral v h_v_mem_vars)
+    some (Literal.mk ⟨v, h_v_mem_vars⟩ ¬ρ v h_v_mem_vars)
   else
     none
 
-@[aesop unsafe]
+@[aesop unsafe, grind →]
 lemma Assignment.negVariable_variable {vars} {ρ : Assignment vars} {v : Variable}
     {y : Literal vars} (h : y ∈ Assignment.negVariable ρ v) : y.variable = v := by
-  unfold Assignment.negVariable at h
   aesop
 
-@[aesop unsafe]
+@[aesop unsafe, grind .]
 lemma Assignment.negVariable_inj {vars} {ρ : Assignment vars} {x₁ x₂ : Variable} {y : Literal vars}
     (h_y_in_mp_x1 : y ∈ ρ.negVariable x₁) (h_y_in_mp_x2 : y ∈ ρ.negVariable x₂) : x₁ = x₂ := by
   grind [Assignment.negVariable, Variable.toLiteral, Variable.toNegLiteral]
-
-@[simp]
-lemma Assignment.negVariable_some_iff_variable_in_vars {vars} {ρ : Assignment vars} {v} :
-    (ρ.negVariable v).isSome ↔ v ∈ vars := by
-  grind [Assignment.negVariable]
 
 /-- The assignment to clause conversion function. -/
 def Assignment.toClause {vars} (ρ : Assignment vars) : Clause vars :=
@@ -43,21 +35,21 @@ def Assignment.toClause {vars} (ρ : Assignment vars) : Clause vars :=
 lemma Assignment.in_toClause {vars} (ρ : Assignment vars) (l : Literal vars) :
     l ∈ ρ.toClause ↔ (l.variable ∈ vars ∧ l.eval ρ = false) := by
   unfold Assignment.toClause
-  simp only [Finset.mem_filterMap, Literal.variable_mem_vars, true_and]
+  simp only [Finset.mem_filterMap]
   constructor
-  case mpr =>
-    intro h_l_in_toClause
-    use l.variable
-    unfold Assignment.negVariable Literal.variable
-    unfold Literal.eval at h_l_in_toClause
-    aesop
-  case mp =>
-    grind [Assignment.negVariable, Variable.toLiteral, Variable.toNegLiteral, Literal.eval]
+  · aesop (add safe unfold Literal.eval)
+  intro ⟨h_var, h_eval⟩
+  use l.variable
+  unfold Assignment.negVariable
+  unfold Literal.eval at h_eval
+  simp_all [↓reduceDIte]
+  rw [←Literal.eq_iff_variable_and_polarity_eq]
+  · grind
 
 @[simp]
 lemma Assignment.toClause_eval {vars} (ρ : Assignment vars) : ρ.toClause.eval ρ = false := by
-  grind [Assignment.toClause, Clause.eval_eq_false_iff_all_falsified_literals,
-  Assignment.negVariable, Literal.eval, Variable.toLiteral, Variable.toNegLiteral]
+  rw [Clause.eval_eq_false_iff_all_falsified_literals]
+  aesop
 
 @[simp]
 lemma Assignment.toClause_variables {vars} (ρ : Assignment vars) : ρ.toClause.variables = vars := by
@@ -65,12 +57,7 @@ lemma Assignment.toClause_variables {vars} (ρ : Assignment vars) : ρ.toClause.
   ext v
   refine ⟨fun a => by aesop, fun h_v_in_vars => ?_⟩
   rw [Finset.mem_image]
-  use (ρ.negVariable v).get <| by rwa [negVariable_some_iff_variable_in_vars]
-  constructor
-  · rw [in_toClause]
-    constructor
-    · simp [Literal.variable_mem_vars]
-    · grind [Assignment.negVariable, Variable.toLiteral, Variable.toNegLiteral, Literal.eval]
-  · aesop
+  use (ρ.negVariable v).get <| by aesop
+  aesop (add safe unfold Literal.eval)
 
 #lint
